pulse/lib/steel/pulse/Pulse.Checker.Abs.fsti
@@ -9,8 +9,5 @@ open Pulse.Checker.Common
 val check_abs
   (g:env)
   (t:st_term{Tm_Abs? t.term})
-  (pre:term)
-  (pre_typing:tot_typing g pre tm_vprop)
-  (post_hint:post_hint_opt g)
   (check:check_t)
-  : T.Tac (checker_result_t g pre post_hint)
+  : T.Tac (t:st_term & c:comp & st_typing g t c)
